First practice tactic completed

src/Practice/practice1.lean
@@ -30,7 +30,7 @@ meta def merge : match_info → match_info → tactic match_info
       else failed
 
 meta def match_expr : expr → expr → tactic match_info
-| `(expr.app %%a₁ %%a₂) `(expr.app %%b₁ %%b₂) :=
+| (expr.app a₁ a₂) (expr.app b₁ b₂) :=
   do m₁ ← match_expr a₁ b₁,
      m₂ ← match_expr a₂ b₂,
      merge m₁ m₂
@@ -38,6 +38,34 @@ meta def match_expr : expr → expr → tactic match_info
   return {limit := n + 1, mapping := λ m, if m = n then t else none }
 | t₁                    t₂                    :=
   if t₁ = t₂ then return {limit := 0, mapping := λ _, none} else failed
+
+meta def find_element_of_type (t : expr) : tactic expr :=
+-- searches for an element of given type in the local context.
+-- Fails if it can't find one.
+do l ← local_context,
+  first $ l.map (λ h,
+    (infer_type h >>= (unify t) >> return h))
+
+meta def build_term (m : match_info) : ℕ → expr → expr → tactic expr
+/- arguments to build_term
+  d : ℕ the depth, how many nested ∃ there are
+  h : expr the term built so far
+  t : expr the type of the term we are trying to build
+-/
+| 0            h t := return h
+| (nat.succ n) h t := do match t with
+  | `(Exists %%motive) :=
+  do e ← match m.mapping n with
+    | (some e) := return e
+    | none     := match motive with
+      | `(λ _ : %%search_type, _) := find_element_of_type search_type
+      | _ := failed end end,
+  previous_t ← whnf (expr.app motive e),
+  term ← build_term n h previous_t,
+  a ← to_expr ```(@Exists.intro _ %%motive %%e %%term),
+  return a
+  | _ := failed
+  end
 
 meta def main_tactic : tactic unit :=
 do t ← target,
@@ -47,12 +75,25 @@ do t ← target,
   first $ l.map (λ h,
     do ht ← infer_type h >>= whnf,
     m ← match_expr c ht,
-    trace ht,
-    e ← return (if m.mapping 0 ≠ none then m.mapping 0 else sorry),
-    answer ← mk_mapp ``Exists.intro [none, none, e, some h],
-    exact answer
-    )
+    answer ← (build_term m d h t),
+    exact answer)
 
+meta def tactic.interactive.main_tactic : tactic unit := main_tactic
 
-theorem main {α : Type*} (a : α) (P : α → Prop) (h : P a) : ∃ x, P x :=
+example {α : Type*} (a : α) (P : α → Prop) (h : P a) : ∃ x, P x :=
+by main_tactic
+
+example {α : Type*} (a b: α) (P : α → α → Prop)
+(h : P a b) : ∃ x y, P x y :=
+by main_tactic
+
+example {α : Type*} (a b c: α) (P : α → α → Prop) (f : α → α)
+(h₁ : P (f a) b) (h₂ : P (f c) (f a)) (h₃ : P b c) : ∃ x y, P (f x) y :=
+by main_tactic
+
+example {α : Type*} (a : α) (P : Prop) (h : P) : ∃ (z : α), P :=
+by main_tactic
+
+example {α : Type*} (a b: α) (P : α → α → Prop)
+(h : P a b) : ∃ x y, ∃ (z : α), P x y :=
 by main_tactic
